NuLLReps.thy
@@ -529,6 +529,13 @@ lemma [\<nu>intro]: "\<nu>ShrIdentical N sid1 \<Longrightarrow> \<nu>ShrIdentica
 lemma [\<nu>intro]: "\<nu>Ownership N ow1 \<Longrightarrow> \<nu>Ownership M ow2 \<Longrightarrow> \<nu>Ownership (N \<nuFusion> M) (ow1 \<times>\<^sub>o\<^sub>w ow2)" unfolding \<nu>Ownership_def by simp
 lemma [\<nu>intro]: "\<nu>Zero N z1 \<Longrightarrow> \<nu>Zero M z2 \<Longrightarrow> \<nu>Zero (N \<nuFusion> M) (z1,z2)" unfolding \<nu>Zero_def by simp
 
+lemma [\<nu>intro]: "\<^bold>c\<^bold>a\<^bold>s\<^bold>t x \<tycolon> N \<longmapsto> x' \<tycolon> N' \<^bold>m\<^bold>e\<^bold>a\<^bold>n\<^bold>w\<^bold>h\<^bold>i\<^bold>l\<^bold>e P \<Longrightarrow> \<^bold>c\<^bold>a\<^bold>s\<^bold>t y \<tycolon> M \<longmapsto> y' \<tycolon> M' \<^bold>m\<^bold>e\<^bold>a\<^bold>n\<^bold>w\<^bold>h\<^bold>i\<^bold>l\<^bold>e Q \<Longrightarrow>
+  \<^bold>c\<^bold>a\<^bold>s\<^bold>t (x,y) \<tycolon> N \<nuFusion> M \<longmapsto> (x',y') \<tycolon> N' \<nuFusion> M' \<^bold>m\<^bold>e\<^bold>a\<^bold>n\<^bold>w\<^bold>h\<^bold>i\<^bold>l\<^bold>e P \<and> Q" unfolding Cast_def by auto
+
+abbreviation AutoFusion (infixr "\<nuFusion>''" 70)  where "N \<nuFusion>' M \<equiv> SchemaTag (N \<nuFusion> M)"
+lemma [\<nu>intro]: "\<^bold>c\<^bold>a\<^bold>s\<^bold>t x \<tycolon> N \<nuFusion> M \<longmapsto> x' \<tycolon> N' \<nuFusion> M' \<^bold>m\<^bold>e\<^bold>a\<^bold>n\<^bold>w\<^bold>h\<^bold>i\<^bold>l\<^bold>e P \<Longrightarrow> \<^bold>c\<^bold>a\<^bold>s\<^bold>t x \<tycolon> N \<nuFusion> M \<longmapsto> x' \<tycolon> N' \<nuFusion>' M' \<^bold>m\<^bold>e\<^bold>a\<^bold>n\<^bold>w\<^bold>h\<^bold>i\<^bold>l\<^bold>e P"
+  unfolding Cast_def SchemaTag_def .
+
 section \<open>Tuple\<close>
 
 datatype 'a tuple = Tuple "('a::field_list)"
